Corrected overflow checks, more robust int_width, test-harness

src/limits.c
@@ -1,0 +1,32 @@
+#include <limits.h>
+#include <stdint.h>
+#include <stdio.h>
+
+#if ( LONG_MIN != -9223372036854775808U )
+  #error ("Assertion LONG_MIN == -9223372036854775808 failed")
+#endif
+#if ( LONG_MAX != 9223372036854775807 )
+  #error ("Assertion LONG_MAX == 9223372036854775807 failed")
+#endif
+
+#ifndef INTPTR_MIN 
+  #error "Not Defined"
+#endif
+
+#if (INTPTR_MIN != LONG_MIN)
+  #error
+#endif
+
+#if (INTPTR_MAX != LONG_MAX)
+  #error
+#endif
+
+intptr_t x--
+
+void main() {
+  printf ("%d", SCHAR_MIN);
+   
+  
+  
+}
+
