src/Test_Harness.thy
@@ -1,0 +1,133 @@
+theory Test_Harness
+imports SmallStep Pretty 
+begin
+
+  datatype test_instr = 
+    Discover string nat
+  | Assert_Eq string int_val   
+  | Assert_Eq_Null string
+  | Assert_Eq_Ptr string nat
+
+  fun adjust_addr :: "int \<Rightarrow> string \<Rightarrow> string" 
+    -- \<open>Adjust address to beginning of its block\<close>
+    where
+    "adjust_addr ofs ca = shows_binop (shows ca) (''-'') (shows ofs) ''''"
+
+  definition ofs_addr :: "int \<Rightarrow> string \<Rightarrow> string"
+    where 
+    "ofs_addr ofs ca = shows_binop (shows ca) (''+'') (shows ofs) ''''"
+
+  definition base_var_name :: "nat \<Rightarrow> string" where
+    "base_var_name i \<equiv> ''__test_harness_x_'' @ show i"
+
+  definition follow :: "string \<Rightarrow> string" where
+    "follow ca \<equiv> ''__TEST_HARNESS_FOLLOW (''@ ca @ '')''"
+
+  term fold
+
+  term list_size
+  thm fold.simps
+
+
+  partial_function (option) fold_option :: "('a \<Rightarrow> 's \<rightharpoonup> 's) \<Rightarrow> 'a list \<Rightarrow> 's \<rightharpoonup> 's" where
+    "fold_option f l s = (case l of 
+        [] \<Rightarrow> Some s 
+      | x#xs \<Rightarrow> do {
+          s \<leftarrow> f x s;
+          fold_option f xs s
+        })"
+
+  lemma fold_option_simps[code,simp]:
+    "fold_option f [] s = Some s"      
+    "fold_option f (x#xs) s = do {
+          s \<leftarrow> f x s;
+          fold_option f xs s
+        }"      
+    by (subst fold_option.simps; simp)+
+
+
+  lemma fold_option_mono[partial_function_mono]:     
+  assumes [partial_function_mono]: "\<And>x \<sigma>. mono_option (\<lambda>fa. f fa x \<sigma>)"
+  shows "mono_option (\<lambda>x. fold_option (f x) l \<sigma>)"
+    apply (induction l arbitrary: \<sigma>)
+    apply simp
+    apply (tactic \<open>Partial_Function.mono_tac @{context} 1\<close>)
+    apply simp
+    apply (tactic \<open>Partial_Function.mono_tac @{context} 1\<close>)
+    apply simp
+    done
+
+  context fixes \<mu> :: mem begin  
+
+  partial_function (option) dfs 
+    :: "nat set \<Rightarrow> addr \<Rightarrow> string \<Rightarrow> (nat set \<times> test_instr list) option"
+    where
+    [code]: "dfs D a ca = do {
+      let (base,ofs) = a;
+
+      case \<mu>!base of
+        None \<Rightarrow> Some (D,[])
+      | Some b \<Rightarrow> do {  
+          let ca = adjust_addr ofs ca;
+          if base \<notin> D then do {
+            let D = insert base D;
+            let emit = [Discover ca base];
+            
+            fold_option (\<lambda>i (D,emit). do {
+              let i=int i;
+              let cai = (ofs_addr i (base_var_name base));
+              case b!!i of
+                None \<Rightarrow> Some (D,emit)
+              | Some (I v) \<Rightarrow> Some (D,emit @ [Assert_Eq cai v])
+              | Some (NullVal) \<Rightarrow> Some (D,emit @ [Assert_Eq_Null cai] )
+              | Some (A addr) \<Rightarrow> do {
+                  (D,emit')\<leftarrow>dfs D addr (follow cai);
+                  Some (D,emit@emit')
+                }
+            })
+              [0..<length b]
+              (D,emit)
+
+          } else do {
+            Some (D,[Assert_Eq_Ptr ca base])
+          }
+        }    
+    }"
+
+  end
+
+  definition emit_globals_tests :: "vname list \<Rightarrow> state \<rightharpoonup> (nat set \<times> test_instr list)" where
+    "emit_globals_tests \<equiv> \<lambda>vnames (\<sigma>,\<gamma>,\<mu>). 
+      fold_option (\<lambda>x (D,emit). do {
+        case \<gamma> x of
+          Some vo \<Rightarrow> do {
+            let cai = x;
+            case vo of
+                None \<Rightarrow> Some (D,emit)
+              | Some (I v) \<Rightarrow> Some (D,emit @ [Assert_Eq cai v])
+              | Some (NullVal) \<Rightarrow> Some (D,emit @ [Assert_Eq_Null cai] )
+              | Some (A addr) \<Rightarrow> do {
+                  (D,emit')\<leftarrow>dfs \<mu> D addr (follow cai);
+                  Some (D,emit@emit')
+                }
+          }
+        | _ \<Rightarrow> Some (D,emit)
+      }
+      ) vnames ({},[])"
+
+  definition tests_variables :: "test_instr list \<Rightarrow> shows" where
+    "tests_variables l \<equiv> foldr (\<lambda>                   
+      (Discover _ i) \<Rightarrow> shows dflt_type o shows '' *'' o shows (base_var_name i) o shows '';'' o shows_nl
+      | _ \<Rightarrow> id
+      ) l"
+
+  definition tests_instructions :: "test_instr list \<Rightarrow> shows" where
+    "tests_instructions l \<equiv> foldr (\<lambda>                   
+        (Discover ca i) \<Rightarrow> shows ''__TEST_HARNESS_DISCOVER '' o shows_paren ( shows ca o shows '', '' o shows (base_var_name i)) o shows_nl
+      | (Assert_Eq ca v) \<Rightarrow> shows ''__TEST_HARNESS_ASSERT_EQ '' o shows_paren ( shows ca o shows '', '' o shows v) o shows_nl
+      | (Assert_Eq_Null ca) \<Rightarrow> shows ''__TEST_HARNESS_ASSERT_EQ_NULL '' o shows_paren ( shows ca ) o shows_nl
+      | (Assert_Eq_Ptr ca i) \<Rightarrow> shows ''__TEST_HARNESS_ASSERT_EQ_PTR '' o shows_paren ( shows ca o shows '', '' o shows (base_var_name i)) o shows_nl
+      ) l"
+
+
+end
